proof/capDL-api/Retype_DP.thy
@@ -8,58 +8,32 @@ theory Retype_DP
 imports Invocation_DP
 begin
 
-lemma create_objects_mapM_x:
-  "create_objects ids (Some obj) = mapM_x (\<lambda>id. create_objects [id] (Some obj)) ids "
-  proof (induct ids)
-    case Nil
-    show ?case
-      by (simp add:create_objects_def mapM_x_Nil simpler_modify_def return_def)
-  next
-    case Cons
-    show ?case
-      apply (simp add:mapM_x_Cons)
-      apply (subst local.Cons[symmetric])
-      apply (rule ext)
-      apply (case_tac x)
-      apply (clarsimp simp:create_objects_def simpler_modify_def bind_def)
-      apply (rule ext)
-      apply clarsimp
-    done
-qed
-
 lemma create_objects_mapM_x':
   "ids = map (\<lambda>x. {x}) ids' \<Longrightarrow>
-  create_objects ids (Some obj) = mapM_x (\<lambda>id. create_objects [{id}] (Some obj)) ids' "
-  apply simp
-  proof (induct ids' arbitrary: ids)
-    case Nil
-    show ?case
-      by (simp add:create_objects_def mapM_x_Nil simpler_modify_def return_def)
-  next
-    case Cons
-    show ?case
-      apply (simp add:mapM_x_Cons)
-      apply (subst local.Cons[symmetric])
-       apply simp
-      apply (rule ext)
-      apply (case_tac x)
-      apply (clarsimp simp:create_objects_def simpler_modify_def bind_def)
-      apply (rule ext)
-      apply clarsimp
+   create_objects ids (Some obj) = mapM_x (\<lambda>id. create_objects [{id}] (Some obj)) ids'"
+proof (simp, induct ids' arbitrary: ids)
+  case Nil
+  show ?case
+    by (simp add: create_objects_def mapM_x_Nil simpler_modify_def return_def)
+next
+  case Cons
+  show ?case
+    apply (simp add: mapM_x_Cons)
+    apply (subst local.Cons[symmetric])
+     apply simp
+    apply (rule ext, rename_tac x)
+    apply (case_tac x)
+    apply (clarsimp simp: create_objects_def simpler_modify_def bind_def)
+    apply (rule ext)
+    apply clarsimp
     done
 qed
 
-lemma pick_rev:
-  assumes "target_object_ids = map (\<lambda>x. {x}) ids"
-  shows "ids = map (\<lambda>x. pick x) target_object_ids"
-  unfolding assms by (induct ids) auto
-
 lemma create_objects_wp:
-  notes set_map[simp del]
-  shows
-  "\<lbrace> K (obj_refs = map (\<lambda>x. {x}) (map pick obj_refs) \<and> distinct (map pick obj_refs) )
-  and <(\<And>* ptr\<in>pick ` set obj_refs. ptr \<mapsto>o Untyped) \<and>* P > \<rbrace>
-  create_objects obj_refs (Some obj) \<lbrace>\<lambda>r s. <(\<And>* ptr\<in>pick ` set obj_refs. ptr \<mapsto>o obj) \<and>* P > s \<rbrace>"
+  "\<lbrace> K (obj_refs = map (\<lambda>x. {x}) (map pick obj_refs) \<and> distinct (map pick obj_refs) ) and
+     <(\<And>* ptr\<in>pick ` set obj_refs. ptr \<mapsto>o Untyped) \<and>* P> \<rbrace>
+   create_objects obj_refs (Some obj)
+   \<lbrace>\<lambda>r s. <(\<And>* ptr\<in>pick ` set obj_refs. ptr \<mapsto>o obj) \<and>* P > s \<rbrace>"
   apply (rule hoare_name_pre_state)
   apply (subst create_objects_mapM_x'[where ids' = "map pick obj_refs"])
    apply simp
@@ -69,36 +43,21 @@ lemma create_objects_wp:
    apply (rule create_one_wp)
    apply (subst set_map[symmetric])
    apply (subst sep_list_conj_sep_map_set_conj[symmetric])
-    apply (simp add:distinct_map)
+    apply (simp add: distinct_map)
    apply simp
-  apply (clarsimp simp: set_map[symmetric])
+  apply (clarsimp simp flip: set_map)
   apply (subst(asm) sep_list_conj_sep_map_set_conj[symmetric])
-   apply (simp add:distinct_map)
-  apply (simp add:set_map)
+   apply (simp add: distinct_map)
   apply sep_cancel
   apply (erule sep_list_conj_impl[rotated])
-  apply (simp add:list_all2_iff)
-  apply (clarsimp simp:zip_map1 zip_map2
-    set_zip_same
-    Fun.comp_def split_def)
-  proof (induct obj_refs)
-    case Nil
-    show ?case
-      using Nil.prems
-      by simp
-  next
-    case Cons
-    show ?case
-      using Cons.prems
-    apply clarsimp
-    apply (erule disjE)
-     apply (fastforce simp:sep_any_def)
-    apply (erule(3) Cons.hyps)
-    done
-  qed
+  apply (simp add: list_all2_iff)
+  apply (clarsimp simp: zip_map1 zip_map2 set_zip_same Fun.comp_def split_def)
+  apply (induct obj_refs; simp)
+  apply (fastforce simp:sep_any_def)
+  done
 
-lemma nonempty_pick_in:
-  "a\<noteq>{} \<Longrightarrow> pick a \<in> a"
+lemma nonempty_pick_in: (* FIXME: duplicate in drefine/Lemmas_D.thy *)
+  "a \<noteq> {} \<Longrightarrow> pick a \<in> a"
   by (metis all_not_in_conv someI_ex)
 
 lemma retype_region_wp:
@@ -119,25 +78,9 @@ lemma retype_region_wp:
     apply (wp create_objects_wp | simp)+
   done
 
-lemma map_zip_first_simp:
-  "length x = length y \<Longrightarrow> map (\<lambda>a. g (fst a)) (zip x y) = map g x"
-  proof (induct x arbitrary: y)
-    case Nil
-    show ?case
-      by simp
-  next
-    case Cons
-    show ?case
-      using local.Cons.prems
-      apply (case_tac y)
-       apply clarsimp+
-      apply (simp add:local.Cons.hyps)
-    done
-qed
-
 lemma update_range_simple:
-  "idx \<noteq> 0 \<Longrightarrow> ptr \<le> ptr + of_nat idx \<Longrightarrow>
-      update_range old_range ptr idx = old_range - {..<ptr + of_nat idx}"
+  "\<lbrakk> idx \<noteq> 0; ptr \<le> ptr + of_nat idx \<rbrakk> \<Longrightarrow>
+   update_range old_range ptr idx = old_range - {..<ptr + of_nat idx}"
   by (clarsimp simp: update_range_def)
 
 lemma update_available_range_wp:
@@ -150,60 +93,53 @@ lemma update_available_range_wp:
   apply (intro conjI impI; sep_solve)
   done
 
-lemmas update_available_range_wp' = update_available_range_wp
-  [where cap="UntypedCap dev b c" for dev b c, simplified]
-
 lemma reset_cap_asid_untyped_cap_eqD:
-  "reset_cap_asid c = UntypedCap dev a b
-  \<Longrightarrow> c = UntypedCap dev a b"
-  by (simp add:reset_cap_asid_def split:cdl_cap.splits)
+  "reset_cap_asid c = UntypedCap dev a b \<Longrightarrow> c = UntypedCap dev a b"
+  using reset_cap_asid_simps2
+  by blast
 
 lemma dummy_detype_if_untyped:
-  "\<lbrakk>finite obj_range ;<(\<And>* ptr\<in>obj_range. ptr \<mapsto>o Untyped) \<and>* P > s\<rbrakk>
-  \<Longrightarrow> (detype obj_range s) = s"
-  apply (case_tac s,clarsimp simp:detype_def sep_set_conj_def)
-  apply (rule ext)
-  apply (clarsimp simp:sep_state_projection_def sep_conj_def)
+  "\<lbrakk>finite obj_range; <(\<And>* ptr\<in>obj_range. ptr \<mapsto>o Untyped) \<and>* P> s\<rbrakk>
+   \<Longrightarrow> detype obj_range s = s"
+  apply (case_tac s, clarsimp simp:detype_def sep_set_conj_def)
+  apply (rule ext, rename_tac x)
+  apply (clarsimp simp: sep_state_projection_def sep_conj_def)
+  apply (rename_tac x' y)
   apply (subst (asm) sep.prod.remove)
    apply simp+
-  apply (clarsimp simp:sep_map_o_conj image_def)
+  apply (clarsimp simp: sep_map_o_conj image_def)
   apply (drule_tac f = sep_heap in arg_cong)
-  apply (drule_tac x = "(x,Fields)" in fun_cong)+
-  apply (case_tac xa,case_tac y)
-  apply (clarsimp simp:plus_sep_state_def sep_state_add_def asid_reset_def
-    intent_reset_def update_slots_def object_wipe_slots_def sep_disj_sep_state_def
-    object_to_sep_state_def object_project_def object_clean_def
-    sep_state_disj_def)
+  apply (drule_tac x = "(x, Fields)" in fun_cong)+
+  apply (case_tac x', case_tac y)
+  apply (clarsimp simp: plus_sep_state_def sep_state_add_def asid_reset_def sep_disj_sep_state_def
+                        intent_reset_def update_slots_def object_wipe_slots_def sep_state_disj_def
+                        object_to_sep_state_def object_project_def object_clean_def)
   apply (drule map_disj_None_right'[rotated])
    apply simp
-  apply (clarsimp simp: map_add_def split:option.splits)
-  apply (case_tac z)
-    apply (clarsimp simp:plus_sep_state_def sep_state_add_def asid_reset_def
-    intent_reset_def update_slots_def object_wipe_slots_def sep_disj_sep_state_def
-    object_to_sep_state_def object_project_def object_clean_def
-    sep_state_disj_def)+
+  apply (clarsimp simp: map_add_def split: option.splits)
+  apply (rename_tac obj)
+  apply (case_tac obj)
+    apply (clarsimp simp: plus_sep_state_def sep_state_add_def asid_reset_def sep_disj_sep_state_def
+                          intent_reset_def update_slots_def object_wipe_slots_def
+                          object_to_sep_state_def object_project_def object_clean_def
+                          sep_state_disj_def)+
   done
 
 lemma mapME_x_wp:
   "\<forall>x \<in> set xs. \<lbrace>P\<rbrace> f x \<lbrace>\<lambda>rv. P\<rbrace>,\<lbrace>E\<rbrace> \<Longrightarrow> \<lbrace>P\<rbrace> mapME_x f xs \<lbrace>\<lambda>rv. P\<rbrace>,\<lbrace>E\<rbrace>"
-  proof (induct xs)
+proof (induct xs)
   case Nil
   show ?case
-   apply (simp add: mapME_x_def sequenceE_x_def)
-   by wp
-  next
+    by (wpsimp simp: mapME_x_def sequenceE_x_def)
+next
   case Cons
+  then
   show ?case
-   using Cons.prems
-   apply (simp add: mapME_x_def sequenceE_x_def)
-   apply (fold mapME_x_def sequenceE_x_def)
-   including no_pre
-   apply wp
-    apply (rule Cons.hyps)
-    apply fastforce
-   apply fastforce
-   done
-  qed
+    apply (simp add: mapME_x_def sequenceE_x_def)
+    apply (fold mapME_x_def sequenceE_x_def)
+    apply (wp; fastforce)
+    done
+qed
 
 lemma hoare_whenE_not:
   "\<lbrace>\<lambda>s. R () s \<and> \<not>P\<rbrace> whenE P f \<lbrace>R\<rbrace>, \<lbrace>E\<rbrace>"
@@ -221,20 +157,18 @@ lemma reset_untyped_cap_wp_trivial:
   done
 
 lemma reset_untyped_cap_wp_trivial':
-  "\<lbrace><uref \<mapsto>c UntypedCap dev obj_range free_range \<and>* P>
-     and (\<lambda>_. obj_range = free_range)\<rbrace> reset_untyped_cap uref
-    \<lbrace>\<lambda>_. <uref \<mapsto>c UntypedCap dev obj_range free_range \<and>* P>\<rbrace>, -"
+  "\<lbrace><uref \<mapsto>c UntypedCap dev obj_range free_range \<and>* P> and (\<lambda>_. obj_range = free_range)\<rbrace>
+   reset_untyped_cap uref
+   \<lbrace>\<lambda>_. <uref \<mapsto>c UntypedCap dev obj_range free_range \<and>* P>\<rbrace>, -"
   by (wp reset_untyped_cap_wp_trivial)
 
 lemma reset_untyped_cap_wp_trivial'':
-  "\<lbrace><uref \<mapsto>c UntypedCap dev obj_range free_range \<and>* P>
-     and (\<lambda>_. obj_range = free_range) and R ()\<rbrace> reset_untyped_cap uref \<lbrace>\<lambda>y. R y\<rbrace>, -"
+  "\<lbrace><uref \<mapsto>c UntypedCap dev obj_range free_range \<and>* P> and (\<lambda>_. obj_range = free_range) and R ()\<rbrace>
+   reset_untyped_cap uref
+   \<lbrace>R\<rbrace>, -"
   unfolding validE_R_def
-  apply (rule hoare_name_pre_stateE)
-  apply (clarsimp simp: reset_untyped_cap_def)
+  apply (wpsimp wp: hoare_whenE_not mapME_x_wp simp: reset_untyped_cap_def)
   apply (sep_frule (direct) opt_cap_sep_imp, clarsimp dest!: reset_cap_asid_untyped_cap_eqD)
-  apply (wp hoare_whenE_not mapME_x_wp)
-  apply (clarsimp)
   done
 
 crunch reset_untyped_cap
@@ -256,89 +190,96 @@ lemma create_cap_wp:
   apply sep_solve
   done
 
-(* FIXME: move to sep-CapDL  *)
+(* FIXME: move to sep-capDL  *)
 lemma sep_lift_generic:
-  "\<And>sep_lift.
-   (\<And>R. \<lbrace>g (R)\<rbrace> f \<lbrace>\<lambda>x s. (P x \<and>* R) (sep_lift s)\<rbrace>) \<Longrightarrow>
-     \<lbrace>g (ALLS x. P x \<longrightarrow>* R x)\<rbrace> f \<lbrace>\<lambda>rv s . R rv (sep_lift s)\<rbrace>"
-  apply (rule hoare_chain, assumption)+
-   apply (fastforce)
+  "(\<And>R. \<lbrace>g (R)\<rbrace> f \<lbrace>\<lambda>x s. (P x \<and>* R) (sep_lift s)\<rbrace>) \<Longrightarrow>
+   \<lbrace>g (ALLS x. P x \<longrightarrow>* R x)\<rbrace> f \<lbrace>\<lambda>rv s . R rv (sep_lift s)\<rbrace>"
+  apply (rule hoare_chain, assumption)
+   apply fastforce
   apply (clarsimp simp: sep_conj_def)
-  using sep_add_commute sep_disj_commuteI sep_implD by fastforce
+  using sep_add_commute sep_disj_commuteI sep_implD
+  apply fastforce
+  done
 
-(* FIXME: move to sep-CapDL  *)
+(* FIXME: move to sep-capDL  *)
 lemma sep_lift_generic_E:
-  "\<And>sep_lift.
-   (\<And>R. \<lbrace>g (R)\<rbrace> f \<lbrace>\<lambda>x s. (P x \<and>* R) (sep_lift s)\<rbrace>, \<lbrace>E\<rbrace>) \<Longrightarrow>
-     \<lbrace>g (ALLS x. P x \<longrightarrow>* R x)\<rbrace> f \<lbrace>\<lambda>rv s . R rv (sep_lift s)\<rbrace>, \<lbrace>E\<rbrace>"
+  "(\<And>R. \<lbrace>g (R)\<rbrace> f \<lbrace>\<lambda>x s. (P x \<and>* R) (sep_lift s)\<rbrace>, \<lbrace>E\<rbrace>) \<Longrightarrow>
+   \<lbrace>g (ALLS x. P x \<longrightarrow>* R x)\<rbrace> f \<lbrace>\<lambda>rv s . R rv (sep_lift s)\<rbrace>, \<lbrace>E\<rbrace>"
   unfolding validE_R_def
-  apply (rule hoare_chainE, assumption)+
-    apply (fastforce)
+  apply (rule hoare_chainE, assumption)
+    apply fastforce
    apply (clarsimp simp: sep_conj_def)
-  using sep_add_commute sep_disj_commuteI sep_implD apply fastforce
-  by (simp)
+   using sep_add_commute sep_disj_commuteI sep_implD
+   apply fastforce
+  apply simp
+  done
 
+(* FIXME: move to sep-capDL  *)
 lemma sep_lift_generic_R:
-  "\<And>sep_lift.
-   (\<And>R. \<lbrace>g (R)\<rbrace> f \<lbrace>\<lambda>x s. (P x \<and>* R) (sep_lift s)\<rbrace>, -) \<Longrightarrow>
-     \<lbrace>g (ALLS x. P x \<longrightarrow>* R x) \<rbrace> f \<lbrace>\<lambda>rv s . R rv (sep_lift s) \<rbrace>, -"
+  "(\<And>R. \<lbrace>g (R)\<rbrace> f \<lbrace>\<lambda>x s. (P x \<and>* R) (sep_lift s)\<rbrace>, -) \<Longrightarrow>
+   \<lbrace>g (ALLS x. P x \<longrightarrow>* R x) \<rbrace> f \<lbrace>\<lambda>rv s . R rv (sep_lift s) \<rbrace>, -"
   unfolding validE_R_def
   by (rule sep_lift_generic_E, simp)
 
-lemma distinct_pick: "\<lbrakk>distinct xs;  \<forall>s\<in>set xs. \<exists>v. {v} = s\<rbrakk> \<Longrightarrow> distinct (map pick xs)"
-  apply (induct xs; clarsimp?)
-  apply (clarsimp simp: Ball_def)
-  apply (erule_tac x=aa in allE)
-  apply (clarsimp simp: pick_def)
-  done
+lemma distinct_pick:
+  "\<lbrakk>distinct xs; \<forall>S\<in>set xs. \<exists>v. {v} = S\<rbrakk> \<Longrightarrow> distinct (map pick xs)"
+  by (induct xs; clarsimp)
+     (fastforce simp: Ball_def)
 
-lemma distinct_singleton_union_eq: "\<lbrakk>distinct xs; \<forall>s\<in>set xs. \<exists>v. {v} = s\<rbrakk>
-     \<Longrightarrow>  \<Union> (set xs) = pick ` (set xs)"
+lemma distinct_singleton_union_eq:
+  "\<lbrakk>distinct xs; \<forall>S\<in>set xs. \<exists>v. {v} = S\<rbrakk> \<Longrightarrow> \<Union> (set xs) = pick ` (set xs)"
   by (induct xs; clarsimp)
 
-lemma map_zip_helper: "map (\<lambda>x. f (fst x)) (zip xs ys) = map f (take (length ys) xs)"
-  apply (induct xs arbitrary: ys ; clarsimp?)
-  apply (case_tac ys; clarsimp)
-done
+lemma map_fst_zip_helper: (* FIXME: move to Lib *)
+  "map (\<lambda>x. f (fst x)) (zip xs ys) = map f (take (length ys) xs)"
+  apply (induct xs arbitrary: ys; clarsimp?)
+  apply (rename_tac ys, case_tac ys; clarsimp)
+  done
 
-lemma map_zip_helper': "map (\<lambda>x. f (fst x)) (zip xs (map g [0..<length xs])) = map f xs"
-  apply (induct xs; clarsimp)
-  apply (subst map_zip_helper, clarsimp)
-done
+(* FIXME: move; consider moving next 3 to Lib *)
+lemma fst_case_prod[simp]:
+  "fst (case v of (x, y) \<Rightarrow> (f x, g y)) = f (fst v) "
+  by (simp add: case_prod_unfold)
 
-lemma [simp]: "fst (case v of (x, y) \<Rightarrow> (f x, g y)) = ((f (fst v))) "
- by (cases v, simp)
+lemma snd_case_prod[simp]:
+  "snd (case v of (x, y) \<Rightarrow> (f x, g y)) = g (snd v)"
+  by (simp add: case_prod_unfold)
 
-lemma [simp]: "snd (case v of (x, y) \<Rightarrow> (f x, g y)) = ((g (snd v))) "
- by (cases v, simp)
+lemma case_prod_of_case_prod[simp]:
+  "(case case v of (x, y) \<Rightarrow> (f x, g y) of (x', y') \<Rightarrow> f' x' y') = f' (f (fst v)) (g (snd v))"
+  by (simp add: case_prod_unfold)
 
-lemma [simp]: "(case case v of (x, y) \<Rightarrow> (f x, g y) of (x', y') \<Rightarrow> f' x' y') = ( f' (f (fst v)) (g (snd v)))"
- by (cases v, clarsimp)
+(* These terms below occur a lot in retype proofs. Abbreviate to make the goals more readable. *)
+abbreviation
+  "aligned_min_of r1 r2 nt ts \<equiv> alignUp (min_of_range r1 r2) (obj_bits_cdl nt ts)"
+
+abbreviation
+  "cond_min_of P r1 r2 nt ts \<equiv> if P then aligned_min_of r1 r2 nt ts else min_of_range r1 r2"
 
 lemma invoke_untyped_wp:
-  "\<lbrace> K (default_object nt ts minBound = Some obj \<and> nt \<noteq> UntypedType
-     \<and> length slots = n  \<and> (generate_range (aligned_ptr) nt sz n) = created_range
-     \<and> distinct created_range \<and> base_ptr = Min obj_range \<and> sz = (obj_bits_cdl nt ts) \<and>
-     new_idx = unat (aligned_ptr + (of_nat n << sz) - base_ptr)  \<and>
-     (\<not> has_kids \<longrightarrow> aligned_ptr = Min (get_range ((\<noteq>) {}) free_range obj_range))
-     \<and> (has_kids \<longrightarrow> aligned_ptr = alignUp (Min (get_range ((\<noteq>) {}) free_range obj_range)) sz)
-     \<and> (\<not> has_kids \<longrightarrow> free_range = obj_range))
-     and (\<lambda>s. cdl_current_domain s = minBound)
-     and < \<And>* map (\<lambda>dest_slot. dest_slot \<mapsto>c NullCap) slots
-    \<and>*(\<And>* ptr\<in>\<Union> (set created_range). ptr \<mapsto>o Untyped)
-    \<and>* uref \<mapsto>c UntypedCap dev obj_range free_range
-    \<and>* P > \<rbrace>
-  invoke_untyped (Retype uref nt ts slots has_kids n)
-  \<lbrace>\<lambda>_ s.
-  < \<And>* map (\<lambda>(dest_slot, obj_refs). dest_slot \<mapsto>c (default_cap nt obj_refs ts dev)) (zip slots created_range)
-  \<and>* (\<And>* ptr\<in>\<Union> (set created_range). ptr \<mapsto>o obj)
-  \<and>* uref \<mapsto>c UntypedCap dev obj_range (update_range obj_range base_ptr new_idx)
-  \<and>* P > s \<rbrace>, -"
+  "\<lbrace>K (default_object nt ts minBound = Some obj \<and> nt \<noteq> UntypedType
+       \<and> length slots = n  \<and> (generate_range (aligned_ptr) nt sz n) = created_range
+       \<and> distinct created_range \<and> base_ptr = Min obj_range \<and> sz = (obj_bits_cdl nt ts)
+       \<and> new_idx = unat (aligned_ptr + (of_nat n << sz) - base_ptr)
+       \<and> (\<not> has_kids \<longrightarrow> aligned_ptr = min_of_range free_range obj_range)
+       \<and> (has_kids \<longrightarrow> aligned_ptr = alignUp (min_of_range free_range obj_range) sz)
+       \<and> (\<not> has_kids \<longrightarrow> free_range = obj_range)) and
+    (\<lambda>s. cdl_current_domain s = minBound) and
+    <\<And>* map (\<lambda>dest_slot. dest_slot \<mapsto>c NullCap) slots
+     \<and>*(\<And>* ptr\<in>\<Union> (set created_range). ptr \<mapsto>o Untyped)
+     \<and>* uref \<mapsto>c UntypedCap dev obj_range free_range
+     \<and>* P>\<rbrace>
+   invoke_untyped (Retype uref nt ts slots has_kids n)
+   \<lbrace>\<lambda>_.
+     <\<And>* map (\<lambda>(dest_slot, obj_refs). dest_slot \<mapsto>c (default_cap nt obj_refs ts dev))
+              (zip slots created_range)
+      \<and>* (\<And>* ptr\<in>\<Union> (set created_range). ptr \<mapsto>o obj)
+      \<and>* uref \<mapsto>c UntypedCap dev obj_range (update_range obj_range base_ptr new_idx)
+      \<and>* P>\<rbrace>, -"
   apply (simp add: validE_R_def)
   apply (rule hoare_name_pre_stateE)
   apply (clarsimp simp:invoke_untyped_def unless_def)
-  apply (rule hoare_pre)
-   apply wp
+  apply wp
        apply (wp sep_hoare_fold_mapM_x[OF create_cap_wp[where cap=NullCap], simplified])
       apply (wp retype_region_wp[simplified sep_wp_simp, THEN sep_lift_generic])
      apply (wp update_available_range_wp[simplified sep_wp_simp, THEN sep_lift_generic])
@@ -359,16 +300,19 @@ lemma invoke_untyped_wp:
     apply (clarsimp simp: generate_range_def, clarsimp)
    apply (sep_cancel)+
    apply (rule sep_map_sep_foldI)
-   apply (subgoal_tac "(\<And>* map (\<lambda>x. fst x \<mapsto>c NullCap)
-            (zip slots (generate_range (alignUp (Min (get_range ((\<noteq>) {}) free_range obj_range)) (obj_bits_cdl nt ts)) nt (obj_bits_cdl nt ts) (length slots))))
-             = (\<And>* map (\<lambda>x. x \<mapsto>c NullCap) slots)")
-    prefer 2
+   apply (prop_tac "\<And>* map (\<lambda>x. fst x \<mapsto>c NullCap)
+                            (zip slots (generate_range
+                                          (aligned_min_of free_range obj_range nt ts)
+                                          nt
+                                          (obj_bits_cdl nt ts)
+                                          (length slots)))
+                    = \<And>* map (\<lambda>x. x \<mapsto>c NullCap) slots")
     apply (rule arg_cong)
     apply (clarsimp simp: generate_range_def)
-    apply (subst map_zip_helper', simp)
+    apply (subst map_fst_zip_helper, simp)
    apply (clarsimp)
    apply (sep_cancel)+
-   apply (clarsimp simp: generate_range_def zip_map2 map_zip_helper comp_def)
+   apply (clarsimp simp: generate_range_def zip_map2 map_fst_zip_helper comp_def)
   apply (intro impI, clarsimp)
   apply (sep_frule (direct) opt_cap_sep_imp[where p=uref], clarsimp)
   apply (drule reset_cap_asid_untyped_cap_eqD; clarsimp)
@@ -383,51 +327,43 @@ lemma invoke_untyped_wp:
   apply (sep_cancel)+
   apply (rule sep_map_sep_foldI)+
   apply (clarsimp simp: generate_range_def)
-  apply (subst map_zip_helper', sep_cancel+)
-  apply (clarsimp simp: generate_range_def zip_map2 map_zip_helper comp_def)
+  apply (subst map_fst_zip_helper, simp, sep_cancel+)
+  apply (clarsimp simp: generate_range_def zip_map2 map_fst_zip_helper comp_def)
   done
 
 lemma mapME_x_singleton:
   "mapME_x f [a] = (f a >>= return)"
-  by (simp add:mapME_x_def sequenceE_x_def)
+  by (simp add: mapME_x_def sequenceE_x_def)
 
 lemma mapME_singleton:
   "mapME f [a] = (doE x \<leftarrow> f a; returnOk [x] odE)"
   by (simp add:mapME_def sequenceE_def)
 
-
 lemma decode_untyped_invocation_rvu:
-  "\<lbrakk>nt \<noteq> UntypedType\<rbrakk> \<Longrightarrow>
-  \<lbrace> (\<lambda>s. Q (InvokeUntyped (Retype ref nt (unat ts)
-    [(cap_object cnode_cap, unat node_offset)]
-    (has_children ref s) (Suc 0))) s)
-  and R and K(is_cnode_cap cnode_cap)\<rbrace>
-  decode_invocation (UntypedCap dev tot_range free_range) ref [(cnode_cap,cnode_ref)]
-  (UntypedIntent (UntypedRetypeIntent nt ts node_index 0 node_offset 1))
-  \<lbrace>\<lambda>r. Q r\<rbrace>, \<lbrace>\<lambda>r. R\<rbrace>"
-  apply (simp add:decode_invocation_def
-    get_untyped_intent_def throw_opt_def
-    get_index_def throw_on_none_def
-    decode_untyped_invocation_def mapME_x_singleton)
-  apply (rule hoare_pre)
-  apply (wp unlessE_wp
-    lookup_slot_for_cnode_op_rvu' | wpc | clarsimp)+
+  "nt \<noteq> UntypedType \<Longrightarrow>
+   \<lbrace>(\<lambda>s. Q (InvokeUntyped (Retype ref nt (unat ts)
+                                   [(cap_object cnode_cap, unat node_offset)]
+                                   (has_children ref s) (Suc 0))) s)
+    and R and K (is_cnode_cap cnode_cap) \<rbrace>
+   decode_invocation (UntypedCap dev tot_range free_range) ref [(cnode_cap,cnode_ref)]
+                     (UntypedIntent (UntypedRetypeIntent nt ts node_index 0 node_offset 1))
+   \<lbrace>\<lambda>r. Q r\<rbrace>, \<lbrace>\<lambda>r. R\<rbrace>"
+  apply (simp add: decode_invocation_def get_untyped_intent_def throw_opt_def
+                   get_index_def throw_on_none_def decode_untyped_invocation_def mapME_x_singleton)
+  apply (wpsimp wp: lookup_slot_for_cnode_op_rvu')
   done
 
 lemma set_parent_has_children[wp]:
   "\<lbrace>\<top>\<rbrace> set_parent cref uref \<lbrace>\<lambda>r. has_children uref\<rbrace>"
-  apply (clarsimp simp add:set_parent_def simpler_modify_def
-    valid_def has_children_def gets_def assert_def bind_def
-    get_def return_def fail_def)
+  unfolding set_parent_def
+  apply wpsimp
   apply (case_tac cref)
-  apply (auto simp:is_cdt_parent_def)
+  apply (auto simp: is_cdt_parent_def has_children_def)
   done
 
 lemma create_cap_has_children[wp]:
   "\<lbrace>\<top>\<rbrace> create_cap new_type sz uref slot dev \<lbrace>\<lambda>r. has_children uref\<rbrace>"
-  apply (clarsimp simp :create_cap_def split_def)
-  apply wpsimp
-  done
+  by (wpsimp simp: simp: create_cap_def split_def)
 
 crunch retype_region, update_available_range
   for cdt[wp]: "\<lambda>s. P (cdl_cdt s)"
@@ -438,14 +374,19 @@ crunch retype_region, update_available_range
   (simp: crunch_simps corrupt_intents_def has_children_def is_cdt_parent_def)
 
 lemma invoke_untyped_one_has_children:
-  "uinv = (Retype uref nt ts [slot] has_kids (Suc 0))
-  \<Longrightarrow> \<lbrace>K(nt \<noteq> UntypedType)\<rbrace> invoke_untyped uinv \<lbrace>\<lambda>r. has_children uref\<rbrace>,-"
+  "uinv = (Retype uref nt ts [slot] has_kids (Suc 0)) \<Longrightarrow>
+   \<lbrace>K (nt \<noteq> UntypedType)\<rbrace> invoke_untyped uinv \<lbrace>\<lambda>r. has_children uref\<rbrace>, -"
   apply (simp add: invoke_untyped_def)
   apply wp
        apply (rule_tac P = "zip [slot] (generate_range
-                (if has_kids then alignUp (Min (get_range ((\<noteq>) {}) (available_range untyped_cap) (untyped_cap_range untyped_cap))) (obj_bits_cdl nt ts)
-                 else Min (get_range ((\<noteq>) {}) (available_range untyped_cap) (untyped_cap_range untyped_cap)))
-                    nt (obj_bits_cdl nt ts) (Suc 0)) \<noteq> []" in hoare_gen_asm)
+                                          (cond_min_of has_kids
+                                                       (available_range untyped_cap)
+                                                       (untyped_cap_range untyped_cap)
+                                                       nt ts)
+                                          nt
+                                          (obj_bits_cdl nt ts)
+                                          (Suc 0))
+                            \<noteq> []" in hoare_gen_asm)
        apply (rule hoare_strengthen_post[OF mapM_x_accumulate_checks])
          apply (rule create_cap_has_children)
         apply wp
@@ -455,18 +396,16 @@ lemma invoke_untyped_one_has_children:
   done
 
 lemma invoke_untyped_exception:
-  "uinv = (Retype uref nt ts [dest_slot] has_kids (Suc 0))
-  \<Longrightarrow> \<lbrace>K (\<not> has_kids \<longrightarrow> (obj_range = free_range))
-     and < dest_slot \<mapsto>c NullCap \<and>* uref \<mapsto>c UntypedCap dev obj_range free_range
-    \<and>* sep_true > \<rbrace>
+  "uinv = (Retype uref nt ts [dest_slot] has_kids (Suc 0)) \<Longrightarrow>
+   \<lbrace>K (\<not> has_kids \<longrightarrow> obj_range = free_range) and
+    <dest_slot \<mapsto>c NullCap \<and>* uref \<mapsto>c UntypedCap dev obj_range free_range \<and>* sep_true>\<rbrace>
    invoke_untyped uinv
-  -,\<lbrace>\<lambda>r. Q\<rbrace>"
+   -,\<lbrace>\<lambda>r. Q\<rbrace>"
   apply (simp only: invoke_untyped_def validE_E_def)
   apply (rule hoare_name_pre_stateE)
   apply (cases uinv)
   apply clarsimp
-  apply (wp unlessE_wp
-          | wpc | simp add: reset_untyped_cap_def)+
+  apply (wpsimp simp: reset_untyped_cap_def)+
       apply (rule_tac P = "available_range cap = cap_objects cap" in hoare_gen_asmEx)
       apply (simp add: whenE_def)
      apply wp+
@@ -477,32 +416,37 @@ lemma invoke_untyped_exception:
   done
 
 lemma invoke_untyped_one_wp:
-  fixes "free_range" "obj_range" "nt" "ts"
-  defines "aligned_ptr b \<equiv> (if b then alignUp (Min (get_range ((\<noteq>) {}) free_range obj_range)) (obj_bits_cdl nt ts)
-                            else Min (get_range ((\<noteq>) {}) free_range obj_range))"
+  fixes free_range obj_range nt ts
+  defines "aligned_ptr b \<equiv> cond_min_of b free_range obj_range nt ts"
   defines "base_ptr \<equiv> Min obj_range"
   shows
-    "uinv = (Retype uref nt ts [dest_slot] has_kids (Suc 0))
-  \<Longrightarrow> \<lbrace>K (default_object nt ts minBound = Some obj \<and> nt \<noteq> UntypedType
-     \<and> aligned_ptr has_kids \<in> tot_free_range \<and> finite tot_free_range
-     \<and> (\<not> has_kids \<longrightarrow> (obj_range = free_range)))
-     and (\<lambda>s. cdl_current_domain s = minBound)
-     and < dest_slot \<mapsto>c NullCap
-    \<and>* (\<And>* ptr\<in>tot_free_range. ptr \<mapsto>o Untyped)
-    \<and>* uref \<mapsto>c UntypedCap dev obj_range free_range
-    \<and>* P > \<rbrace>
-  invoke_untyped uinv
-  \<lbrace>\<lambda>_ s.
-  < dest_slot \<mapsto>c (default_cap nt {aligned_ptr has_kids} ts dev)
-  \<and>* aligned_ptr has_kids \<mapsto>o obj
-  \<and>* (\<And>* ptr\<in>tot_free_range - {aligned_ptr has_kids}. ptr \<mapsto>o Untyped)
-  \<and>* uref \<mapsto>c UntypedCap dev obj_range (update_range obj_range base_ptr (unat (aligned_ptr has_kids + (1 << obj_bits_cdl nt ts) - base_ptr)))
-  \<and>* P > s \<rbrace>, -"
+    "uinv = (Retype uref nt ts [dest_slot] has_kids (Suc 0)) \<Longrightarrow>
+     \<lbrace>K (default_object nt ts minBound = Some obj \<and> nt \<noteq> UntypedType
+         \<and> aligned_ptr has_kids \<in> tot_free_range \<and> finite tot_free_range
+         \<and> (\<not> has_kids \<longrightarrow> obj_range = free_range)) and
+      (\<lambda>s. cdl_current_domain s = minBound) and
+      <dest_slot \<mapsto>c NullCap
+       \<and>* (\<And>* ptr\<in>tot_free_range. ptr \<mapsto>o Untyped)
+       \<and>* uref \<mapsto>c UntypedCap dev obj_range free_range
+       \<and>* P>\<rbrace>
+     invoke_untyped uinv
+     \<lbrace>\<lambda>_ s.
+        <dest_slot \<mapsto>c (default_cap nt {aligned_ptr has_kids} ts dev)
+         \<and>* aligned_ptr has_kids \<mapsto>o obj
+         \<and>* (\<And>* ptr\<in>tot_free_range - {aligned_ptr has_kids}. ptr \<mapsto>o Untyped)
+         \<and>* uref \<mapsto>c UntypedCap dev obj_range
+                                (update_range obj_range base_ptr
+                                              (unat (aligned_ptr has_kids +
+                                                     (1 << obj_bits_cdl nt ts) - base_ptr)))
+         \<and>* P> s\<rbrace>, -"
   apply simp
-  apply (wp invoke_untyped_wp [where free_range = free_range and obj_range = obj_range and
-                                     aligned_ptr="aligned_ptr has_kids" and sz = "obj_bits_cdl nt ts" and
-                                     obj = obj and base_ptr = base_ptr,
-                                     simplified sep_wp_simp, THEN sep_lift_generic_R])
+  apply (wp invoke_untyped_wp[where free_range = free_range and
+                                    obj_range = obj_range and
+                                    aligned_ptr = "aligned_ptr has_kids" and
+                                    sz = "obj_bits_cdl nt ts" and
+                                    obj = obj and
+                                    base_ptr = base_ptr,
+                                    simplified sep_wp_simp, THEN sep_lift_generic_R])
   apply (clarsimp simp: base_ptr_def)
   apply (rule conjI, simp)
   apply (clarsimp simp: generate_range_def)
@@ -572,12 +516,11 @@ lemma seL4_Untyped_Retype_sep:
       \<and>* (\<And>* ptr\<in>tot_free_range. ptr \<mapsto>o Untyped)
       \<and>* (root_tcb_id, tcb_cspace_slot) \<mapsto>c root_cnode_cap
       \<and>* (cap_object root_cnode_cap, offset croot root_size) \<mapsto>c root_cnode_cap
-      \<and>* P\<guillemotright>
-     and (\<lambda>s. if has_children (root_cnode,ucptr_slot) (kernel_state s)
-              then aligned_ptr = alignUp (Min (get_range ((\<noteq>) {}) free_range obj_range))
-                                         (obj_bits_cdl nt (unat ts))
-              else obj_range = free_range \<and>
-                   aligned_ptr = Min (get_range ((\<noteq>) {}) free_range obj_range))\<rbrace>
+      \<and>* P\<guillemotright> and
+    (\<lambda>s. if has_children (root_cnode,ucptr_slot) (kernel_state s)
+         then aligned_ptr = aligned_min_of free_range obj_range nt (unat ts)
+         else obj_range = free_range \<and>
+              aligned_ptr = min_of_range free_range obj_range)\<rbrace>
    seL4_Untyped_Retype ucptr nt ts croot node_index 0 ncptr_slot_nat 1
    \<lbrace>\<lambda>err s.
       (\<not>err \<longrightarrow>
@@ -624,66 +567,85 @@ lemma seL4_Untyped_Retype_sep:
                                                         [(root_cnode, ncptr_slot)]
                                                         (has_children (cap_object root_cnode_cap,
                                                                        offset ucptr root_size) s)
-                                                        1)" in hoare_gen_asmEx)
+                                                        1)"
+                     in hoare_gen_asmEx)
         apply (simp only: perform_invocation.simps)
         apply (rule hoare_vcg_conj_elimE[where P=P and P'=P for P, simplified, rotated])
          apply wp
          apply (subst conj_assoc[symmetric])
          apply (rule hoare_vcg_conj_liftE_R)
-          apply (rule_tac
-            invoke_untyped_one_wp
-              [where free_range = free_range
-                and obj_range = obj_range
-                and obj = obj  and dev=dev
-                and tot_free_range = tot_free_range and nt=nt and ts="unat ts"
-                and uref = "(cap_object root_cnode_cap, offset ucptr root_size)"
-                and dest_slot = "(cap_object root_cnode_cap, offset ncptr root_size)", simplified sep_wp_simp, THEN sep_lift_generic_R, simplified])
-          apply clarsimp+
-          apply (rule_tac s="has_children (cap_object root_cnode_cap, offset ucptr root_size) s" in trans,
-                  solves simp, rule refl)
-         apply (wp invoke_untyped_one_has_children[where nt=nt and ts="unat ts" and slot="(cap_object root_cnode_cap, offset ncptr root_size)"])
-         apply clarsimp+
-         apply (rule_tac s="has_children (cap_object root_cnode_cap, offset ucptr root_size) s" in trans,
+          apply (rule invoke_untyped_one_wp[
+                        where free_range = free_range
+                          and obj_range = obj_range
+                          and obj = obj
+                          and dev = dev
+                          and tot_free_range = tot_free_range
+                          and nt = nt
+                          and ts = "unat ts"
+                          and uref = "(cap_object root_cnode_cap, offset ucptr root_size)"
+                          and dest_slot = "(cap_object root_cnode_cap, offset ncptr root_size)",
+                        simplified sep_wp_simp, THEN sep_lift_generic_R, simplified])
+          apply clarsimp
+          apply (rule_tac s = "has_children (cap_object root_cnode_cap, offset ucptr root_size) s"
+                          in trans,
                  solves simp, rule refl)
+         apply (wp invoke_untyped_one_has_children[where
+                     nt = nt and
+                     ts = "unat ts" and
+                     slot = "(cap_object root_cnode_cap, offset ncptr root_size)"])
+         apply clarsimp
+         apply (rule_tac s = "has_children (cap_object root_cnode_cap, offset ucptr root_size) s"
+                         in trans,
+                solves simp, rule refl)
         apply (rule hoare_pre)
-         apply (rule_tac has_kids = "(has_children (cap_object root_cnode_cap, offset ucptr root_size) s)" in
-              invoke_untyped_exception[where dest_slot="(cap_object root_cnode_cap, offset ncptr root_size)" and uref="(cap_object root_cnode_cap, offset ucptr root_size)" and nt=nt and ts="unat ts" and free_range = free_range and obj_range = obj_range])[1]
-         apply (clarsimp)
-        apply (clarsimp)
-        apply (sep_solve)
-       apply (wp)
+         apply (rule_tac has_kids = "has_children (cap_object root_cnode_cap,
+                                                   offset ucptr root_size) s"
+                         in invoke_untyped_exception[where
+                              dest_slot = "(cap_object root_cnode_cap, offset ncptr root_size)" and
+                              uref = "(cap_object root_cnode_cap, offset ucptr root_size)" and
+                              nt = nt and
+                              ts = "unat ts" and
+                              free_range = free_range and
+                              obj_range = obj_range])
+         apply clarsimp
+        apply clarsimp
+        apply sep_solve
+       apply wp
        apply (wp set_cap_wp[simplified sep_wp_simp, THEN sep_lift_generic, simplified])
-      apply (rule_tac P =" nt \<noteq> UntypedType
-       \<and> c = UntypedCap dev obj_range free_range \<and> cs = [(root_cnode_cap,(root_cnode,offset croot root_size))]" in hoare_gen_asmEx)
+      apply (rule_tac P = "nt \<noteq> UntypedType \<and> c = UntypedCap dev obj_range free_range \<and>
+                           cs = [(root_cnode_cap,(root_cnode,offset croot root_size))]"
+                      in hoare_gen_asmEx)
       apply (simp only:)
       apply (wp decode_untyped_invocation_rvu)
-      apply (clarsimp)
-     apply (simp only:lookup_extra_caps_def mapME_singleton)
+      apply clarsimp
+     apply (simp only: lookup_extra_caps_def mapME_singleton)
      apply (rule wp_no_exception_seq)
       apply wp
-     apply (wp lookup_cap_and_slot_rvu[where r = root_size and  cap' = "root_cnode_cap"])[1]
-    apply (wp lookup_cap_and_slot_rvu[where r = root_size and cap=root_cnode_cap and cap' = "UntypedCap dev obj_range free_range"])[1]
-    apply (case_tac "(has_children (cap_object root_cnode_cap, offset ucptr root_size)) s")
-     apply (clarsimp)
+     apply (wp lookup_cap_and_slot_rvu[where r = root_size and cap' = "root_cnode_cap"])
+    apply (wp lookup_cap_and_slot_rvu[where r = root_size and
+                                            cap = root_cnode_cap and
+                                            cap' = "UntypedCap dev obj_range free_range"])
+    apply (case_tac "has_children (cap_object root_cnode_cap, offset ucptr root_size) s")
+     apply clarsimp
      apply (intro conjI allI)
           apply (thin_tac "<P \<and>* Q \<and>* (\<lambda>s. True)> s" for P Q s)
-          apply (sep_cancel)+
+          apply sep_cancel+
           apply (intro conjI; sep_solve)
-         apply (sep_solve)
-        apply (fastforce)
-       apply (clarsimp simp:user_pointer_at_def Let_def word_bits_def)
-       apply (sep_solve)
+         apply sep_solve
+        apply fastforce
+       apply (clarsimp simp: user_pointer_at_def Let_def word_bits_def)
+       apply sep_solve
       apply (clarsimp simp: ep_related_cap_def
                      dest!: reset_cap_asid_simps2 reset_cap_asid_cnode_cap)+
-     apply (clarsimp simp:user_pointer_at_def Let_def word_bits_def)
-     apply (sep_solve)
+     apply (clarsimp simp: user_pointer_at_def Let_def word_bits_def)
+     apply sep_solve
     apply (clarsimp simp: ep_related_cap_def user_pointer_at_def Let_def word_bits_def)
     apply (thin_tac "<P \<and>* Q \<and>* (\<lambda>s. True)> s" for P Q s)
     apply (intro conjI)
-       apply (sep_cancel)+
+       apply sep_cancel+
        apply (rule conjI)
-        apply (sep_solve)+
-   apply (clarsimp simp:ep_related_cap_def)+
+        apply sep_solve+
+   apply (clarsimp simp: ep_related_cap_def)+
    apply (wp update_thread_intent_update)
   apply (intro conjI allI impI,simp_all)
     apply (clarsimp simp:ep_related_cap_def)+
@@ -706,44 +668,6 @@ crunch handle_pending_interrupts
   for cdt_inc[wp]: "\<lambda>s. cdl_cdt s child = parent"
   (wp: simp: crunch_simps)
 
-lemmas gets_the_resolve_cap_sym = gets_the_resolve_cap[symmetric]
-
-lemma unify_failure_cdt_lift:
-  "\<lbrace>\<lambda>s. P (cdl_cdt s)\<rbrace> f \<lbrace>\<lambda>r s. P (cdl_cdt s)\<rbrace>
-  \<Longrightarrow> \<lbrace>\<lambda>s. P (cdl_cdt s)\<rbrace> unify_failure f \<lbrace>\<lambda>r s. Q r s \<longrightarrow> P (cdl_cdt s)\<rbrace>,
-  \<lbrace>\<lambda>r s. Q' r s \<longrightarrow> P (cdl_cdt s)\<rbrace>"
-  apply (simp add:unify_failure_def)
-  including no_pre
-  apply (wp hoare_drop_imps)
-  apply (clarsimp simp:validE_def valid_def)
-  done
-
-lemma validE_def2:
-  "\<lbrace>P\<rbrace> f \<lbrace>Q\<rbrace>, \<lbrace>E\<rbrace> =
-  \<lbrace>P\<rbrace> f \<lbrace>\<lambda>v s. (\<forall>e. v = Inl e \<longrightarrow> E e s) \<and> (\<forall>r. v = Inr r \<longrightarrow> Q r s)\<rbrace>"
-  apply (clarsimp simp:validE_def valid_def)
-  apply (rule iffI)
-   apply clarsimp
-   apply (drule_tac x = s in spec)
-   apply fastforce
-  apply clarsimp
-  apply (drule_tac x = s in spec)
-  apply clarsimp
-  apply (drule_tac x = "(a,b)" in bspec)
-   apply simp
-  apply clarsimp
-  apply (case_tac a)
-   apply clarsimp+
-  done
-
-lemma hoare_drop_impE_R:
-  "\<lbrace>P\<rbrace> f \<lbrace>\<lambda>_. Q\<rbrace> \<Longrightarrow> \<lbrace>P\<rbrace> f \<lbrace>\<lambda>r s. R r s \<longrightarrow> Q s\<rbrace>, -"
-  apply (rule validE_validE_R)
-  apply (clarsimp simp:validE_def valid_def)
-  apply (case_tac a,simp_all)
-  apply fastforce
-  done
-
 crunch block_thread_on_ipc
   for cdt_inc[wp]: "\<lambda>s. P (cdl_cdt s)"
 (wp:hoare_vcg_conj_lift hoare_drop_impE_R
@@ -761,120 +685,79 @@ crunch mark_tcb_intent_error
 (wp:hoare_vcg_conj_lift hoare_drop_impE_R
   simp:crunch_simps)
 
-lemma unify_failure_valid:
-  "\<lbrace>\<lambda>s. P s\<rbrace> f \<lbrace>\<lambda>r s. P s\<rbrace>
-  \<Longrightarrow> \<lbrace>\<lambda>s. P s\<rbrace> unify_failure f \<lbrace>\<lambda>r s. P s\<rbrace>"
-  including no_pre
-  apply (simp add:unify_failure_def)
-  apply (wp hoare_drop_imps)
-  apply (clarsimp simp:validE_def valid_def)
-  done
-
 lemma set_parent_other:
   "\<lbrace>\<lambda>s. cdl_cdt s child = Some parent\<rbrace> set_parent dest uref \<lbrace>\<lambda>_ s. cdl_cdt s child = Some parent\<rbrace>"
-  apply (simp add:set_parent_def)
-  apply wp
-  apply auto
-  done
+  by (wpsimp simp: set_parent_def)
 
 lemma invoke_untyped_cdt_inc[wp]:
   "\<lbrace>\<lambda>s. cdl_cdt s child = Some parent \<rbrace>
   invoke_untyped uinv
   \<lbrace>\<lambda>_ s. cdl_cdt s child = Some parent \<rbrace>"
-  apply (clarsimp simp:invoke_untyped_def)
-  apply (case_tac uinv)
-  apply simp
-  apply (rule hoare_pre)
-  apply (wp unlessE_wp)
-      apply (wp mapM_x_wp[OF _ subset_refl])
-       apply (simp add:create_cap_def)
-        apply (rule hoare_pre)
-        apply (wp set_parent_other unless_wp unlessE_wp
-               | wpc | simp)+
+  apply (clarsimp simp: invoke_untyped_def)
+  apply (case_tac uinv, simp)
+  apply (wpsimp wp: mapM_x_wp[OF _ subset_refl] set_parent_other unless_wp unlessE_wp
+                simp: create_cap_def)
    apply (simp add: reset_untyped_cap_def validE_def sum.case_eq_if)
    apply (rule_tac Q'="\<lambda>r s. cdl_cdt s child = Some parent" in hoare_post_imp)
     apply simp
-   apply (wp whenE_wp mapME_x_inv_wp | simp)+
-  apply (clarsimp simp:detype_def)
+   apply (wpsimp wp: mapME_x_inv_wp)
+  apply (clarsimp simp: detype_def)
   done
 
 lemma invoke_untyped_cdt_inc_R[wp]:
   "\<lbrace>\<lambda>s. cdl_cdt s child = Some parent \<rbrace>
-  invoke_untyped uinv
-  \<lbrace>\<lambda>_ s. cdl_cdt s child = Some parent \<rbrace>, -"
+   invoke_untyped uinv
+   \<lbrace>\<lambda>_ s. cdl_cdt s child = Some parent \<rbrace>, -"
   by wp
 
 lemma object_at_cdl_cdt[simp]:
-  "object_at P ptr (s\<lparr>cdl_cdt := a\<rparr>)
-   = object_at P ptr s"
+  "object_at P ptr (s\<lparr>cdl_cdt := a\<rparr>) = object_at P ptr s"
   by (simp add: object_at_def)
 
 crunch set_parent
   for tcb_intent[wp]: "\<lambda>s. tcb_at' (\<lambda>tcb. P (cdl_tcb_intent tcb)) ptr s"
 
-lemma throw_on_none_wp:
-  "\<lbrace>\<lambda>s. case x of None \<Rightarrow> Q s | Some y \<Rightarrow> P y s\<rbrace> throw_on_none x \<lbrace>P\<rbrace>, \<lbrace>\<lambda>r s. Q s\<rbrace>"
-  apply (rule hoare_pre)
-   apply (clarsimp simp:throw_on_none_def)
-   apply (wp | wpc | simp)+
-  apply auto
-  done
+lemma throw_on_none_wp: (* FIXME: move *)
+  "\<lbrace>\<lambda>s. case x of None \<Rightarrow> Q s | Some y \<Rightarrow> P y s\<rbrace> throw_on_none x \<lbrace>P\<rbrace>, \<lbrace>\<lambda>_. Q\<rbrace>"
+  unfolding throw_on_none_def
+  by wpsimp
+     auto
 
-lemma throw_opt_wp:
-  "\<lbrace>\<lambda>s. case x of None \<Rightarrow> Q s | Some y \<Rightarrow> P y s\<rbrace> throw_opt err x \<lbrace>P\<rbrace>, \<lbrace>\<lambda>r s. Q s\<rbrace>"
-  apply (rule hoare_pre)
-   apply (clarsimp simp:throw_opt_def)
-   apply (wp | wpc | simp)+
-  apply auto
-  done
+lemma throw_opt_wp: (* FIXME: move *)
+  "\<lbrace>\<lambda>s. case x of None \<Rightarrow> Q s | Some y \<Rightarrow> P y s\<rbrace> throw_opt err x \<lbrace>P\<rbrace>, \<lbrace>\<lambda>_. Q\<rbrace>"
+  unfolding throw_opt_def
+  by wpsimp
+     auto
 
 lemma lookup_cap_rvu':
-"\<lbrace>\<lambda>s. (\<forall>c. reset_cap_asid c = reset_cap_asid cap' \<longrightarrow> Q c s) \<and>
-    < (thread,tcb_cspace_slot) \<mapsto>c cnode_cap \<and>*
-    \<box> (r, word_bits) : cnode_cap cap_ptr \<mapsto>u cap' \<and>* R> s\<rbrace>
-     lookup_cap thread cap_ptr
-   \<lbrace>Q\<rbrace>, \<lbrace>Q'\<rbrace> "
+  "\<lbrace>\<lambda>s. (\<forall>c. reset_cap_asid c = reset_cap_asid cap' \<longrightarrow> Q c s) \<and>
+        <(thread,tcb_cspace_slot) \<mapsto>c cnode_cap \<and>*
+         (\<box> (r, word_bits) : cnode_cap cap_ptr \<mapsto>u cap') \<and>* R> s\<rbrace>
+   lookup_cap thread cap_ptr
+   \<lbrace>Q\<rbrace>, \<lbrace>Q'\<rbrace>"
   apply (clarsimp simp: lookup_cap_def)
-  apply (wp lookup_slot_rvu [where cnode_cap=cnode_cap] get_cap_rv)
-  apply (clarsimp)
+  apply (wpsimp wp: lookup_slot_rvu[where cnode_cap=cnode_cap] get_cap_rv)
   apply safe
     apply (clarsimp simp: user_pointer_at_def sep_conj_assoc Let_unfold)
-    apply (sep_solve)
+    apply sep_solve
    apply clarsimp
-  apply (sep_solve)
+  apply sep_solve
   done
 
-crunch  handle_pending_interrupts
-  for cdl_current_thread[wp]: "\<lambda>s. P (cdl_current_thread s)"
-
-crunch  lookup_cap
+crunch  handle_pending_interrupts, lookup_cap
   for cdl_current_thread[wp]: "\<lambda>s. P (cdl_current_thread s)"
   (wp: hoare_drop_imps)
 
-lemma throw_opt_wp_valid:
-  "\<lbrace>P\<rbrace> throw_opt err x \<lbrace>\<lambda>r. P\<rbrace>"
-  apply (rule hoare_pre)
-   apply (clarsimp simp:throw_opt_def)
-   apply (wp | wpc | simp)+
-  done
-
-lemma do_notification_transfer_sep_wp:
-  "\<lbrace> cdl.lift ((thread, tcb_pending_op_slot) \<mapsto>c - \<and>* P)\<rbrace> do_notification_transfer thread
-    \<lbrace>\<lambda>rv. cdl.lift ((thread, tcb_pending_op_slot) \<mapsto>c - \<and>* P)\<rbrace>"
-  apply (simp add: do_notification_transfer_def)
-  apply (rule hoare_pre)
-   apply wp
-   apply (rule hoare_post_imp[rotated])
-   apply (rule set_cap_wp)
-   apply sep_solve
-  apply simp
-  done
-
 lemma update_thread_no_pending:
   "\<lbrace>no_pending and
-    K(\<forall>x. (case cdl_tcb_caps x tcb_pending_op_slot of Some cap \<Rightarrow> \<not> is_pending_cap cap | _ \<Rightarrow> True)\<longrightarrow>
-          (case cdl_tcb_caps (t x) tcb_pending_op_slot of Some cap \<Rightarrow> \<not> is_pending_cap cap | _ \<Rightarrow> True))\<rbrace>
-    update_thread thread_ptr t \<lbrace>\<lambda>rv. no_pending\<rbrace>"
+    K (\<forall>x. (case cdl_tcb_caps x tcb_pending_op_slot of
+              Some cap \<Rightarrow> \<not> is_pending_cap cap
+            | _ \<Rightarrow> True)\<longrightarrow>
+           (case cdl_tcb_caps (t x) tcb_pending_op_slot of
+              Some cap \<Rightarrow> \<not> is_pending_cap cap
+            | _ \<Rightarrow> True))\<rbrace>
+   update_thread thread_ptr t
+   \<lbrace>\<lambda>rv. no_pending\<rbrace>"
   unfolding update_thread_def set_object_def
   apply wpsimp
   apply (fastforce simp: opt_cap_def slots_of_def object_slots_def no_pending_def
@@ -882,9 +765,9 @@ lemma update_thread_no_pending:
   done
 
 lemma update_thread_tcb_at:
-  "\<lbrace>K(\<forall>x. P (t x))\<rbrace>
-    update_thread thread_ptr t \<lbrace>\<lambda>rv. tcb_at' P thread_ptr\<rbrace>"
-  apply (rule hoare_pre)
+  "\<lbrace>K (\<forall>x. P (t x))\<rbrace>
+   update_thread thread_ptr t
+   \<lbrace>\<lambda>_. tcb_at' P thread_ptr\<rbrace>"
   apply (simp add: update_thread_def set_object_def | wp modify_wp | wpc)+
   apply (auto simp: no_pending_def object_at_def)
   done
@@ -892,28 +775,23 @@ lemma update_thread_tcb_at:
 lemma corrupt_intents_no_pending:
   "no_pending s \<Longrightarrow> no_pending (corrupt_intents a b s)"
   apply (clarsimp simp: no_pending_def corrupt_intents_def opt_cap_def slots_of_def)
+  apply (rename_tac oid cap)
   apply (drule_tac x = oid in spec)
   apply (auto split: option.splits cdl_object.splits if_splits
               simp: object_slots_def option.splits)
   done
 
-crunch corrupt_ipc_buffer
-  for no_pending[wp]: no_pending
-  (wp: crunch_wps update_thread_no_pending corrupt_intents_no_pending)
-
-crunch mark_tcb_intent_error
+crunch corrupt_ipc_buffer, mark_tcb_intent_error
   for no_pending[wp]: no_pending
   (wp: crunch_wps update_thread_no_pending corrupt_intents_no_pending)
 
 lemma detype_one_wp:
-  "<obj_id \<mapsto>o - \<and>* R> s
-   \<Longrightarrow> <obj_id \<mapsto>o Untyped \<and>* R> (detype {obj_id} s)"
+  "<obj_id \<mapsto>o - \<and>* R> s \<Longrightarrow> <obj_id \<mapsto>o Untyped \<and>* R> (detype {obj_id} s)"
   apply (clarsimp simp: detype_def sep_any_exist)
   apply (clarsimp simp: sep_state_projection_def sep_map_o_conj sep_any_def)
   apply (rule conjI)
    apply (rule ext)
-    apply (clarsimp simp:object_project_def
-      restrict_map_def object_to_sep_state_def)
+   apply (clarsimp simp: object_project_def restrict_map_def object_to_sep_state_def)
   apply (erule arg_cong[where f = R,THEN iffD1,rotated])
   apply clarsimp
   apply (rule ext)
@@ -925,22 +803,23 @@ lemma detype_insert:
   by (cases s, simp add: detype_def fun_eq_iff)
 
 lemma detype_set_sep_helper:
-  "finite S \<Longrightarrow> <(\<And>* x\<in> S. x \<mapsto>o -) \<and>* R> s
-   \<Longrightarrow> <(\<And>* x \<in> S. x \<mapsto>o Untyped) \<and>* R> (detype S s)"
+  "\<lbrakk> finite S; <(\<And>* x\<in> S. x \<mapsto>o -) \<and>* R> s \<rbrakk> \<Longrightarrow> <(\<And>* x \<in> S. x \<mapsto>o Untyped) \<and>* R> (detype S s)"
 proof (induct arbitrary: R rule: finite_induct)
   case empty
-  show ?case using empty by (simp add: detype_def)
+  then
+  show ?case
+    by (simp add: detype_def)
 next
   case (insert a A)
-  show ?case using insert.hyps(1-2) insert.prems
+  then
+  show ?case
     apply (subst detype_insert)
-    apply (simp add: )
-    apply (subst sep_conj_assoc)
+    apply (simp add: sep_conj_assoc)
     apply (rule detype_one_wp)
     apply (sep_select 2)
     apply (rule insert.hyps(3))
     apply sep_solve
-  done
+    done
 qed
 
 lemma detype_set_wp:
@@ -948,11 +827,7 @@ lemma detype_set_wp:
    \<lbrace><(\<And>* x\<in> S. x \<mapsto>o -) \<and>* R>\<rbrace>
     modify (detype S)
    \<lbrace>\<lambda>_. <(\<And>* x \<in> S. x \<mapsto>o Untyped) \<and>* R>\<rbrace>"
-  apply (clarsimp simp: modify_def)
-  apply wp
-  apply (rule detype_set_sep_helper)
-   apply simp+
-  done
+  by (wp detype_set_sep_helper)
 
 lemma invoke_untyped_preempt:
   "finite obj_range \<Longrightarrow>
@@ -996,41 +871,23 @@ lemma invoke_untyped_preempt:
   apply simp
   done
 
-lemma set_parent_cdt_parent:
-  "\<lbrace>\<lambda>s. cdl_cdt s slot = Some parent\<rbrace> set_parent param_a param_b \<lbrace>\<lambda>_ s. cdl_cdt s slot = Some parent\<rbrace>"
-  apply (simp add: set_parent_def)
-  apply wp
-  apply (clarsimp simp add: )
-  done
-
-lemma set_parent_cdl_parent:
-   "\<lbrace>\<lambda>s. cdl_cdt s slot = Some parent\<rbrace>
-     set_parent slot' parent'
-   \<lbrace>\<lambda>_ s. cdl_cdt s slot = Some parent\<rbrace>"
-   apply (simp add: set_parent_def)
-   apply wp
-   apply clarsimp
-   done
-
 crunch reset_untyped_cap
   for cdl_parent[wp]: "\<lambda>s. cdl_cdt s slot = Some parent"
-   (wp: assert_inv crunch_wps mapME_x_inv_wp
-    simp: crunch_simps detype_def)
+  (wp: assert_inv crunch_wps mapME_x_inv_wp
+   simp: crunch_simps detype_def)
 
 crunch insert_cap_child, corrupt_ipc_buffer,
           corrupt_tcb_intent, update_thread, derive_cap, insert_cap_sibling
   for cdl_parent[wp]: "\<lambda>s. cdl_cdt s slot = Some parent"
-   (wp: crunch_wps set_parent_cdl_parent simp: crunch_simps corrupt_intents_def)
+   (wp: crunch_wps set_parent_other simp: crunch_simps corrupt_intents_def)
 
 lemma transfer_caps_loop_cdl_parent:
-   "\<lbrace>\<lambda>s. cdl_cdt s slot = Some parent\<rbrace>
-     transfer_caps_loop ep rcvr caps dest
+  "\<lbrace>\<lambda>s. cdl_cdt s slot = Some parent\<rbrace>
+   transfer_caps_loop ep rcvr caps dest
    \<lbrace>\<lambda>_ s. cdl_cdt s slot = Some parent\<rbrace>"
-   apply (induct caps arbitrary: dest; clarsimp split del: if_split)
-   apply (rule hoare_pre)
-    apply (wp crunch_wps | assumption
-      | simp add: crunch_simps split del: if_split)+
-   done
+  apply (induct caps arbitrary: dest; clarsimp split del: if_split)
+  apply (wpsimp wp: crunch_wps simp: crunch_simps | assumption)+
+  done
 
 lemmas reset_untyped_cap_cdl2[wp] = reset_untyped_cap_cdl_parent[THEN valid_validE_E]
 
@@ -1039,7 +896,9 @@ crunch inject_reply_cap
   (simp: crunch_simps unless_def wp: crunch_wps)
 
 lemma set_object_no_pending:
-  "\<lbrace>no_pending and K(\<forall>cap. object_slots x tcb_pending_op_slot = Some cap \<longrightarrow> \<not> is_pending_cap cap)\<rbrace> set_object a x \<lbrace>\<lambda>rv. no_pending\<rbrace>"
+  "\<lbrace>no_pending and K (\<forall>cap. object_slots x tcb_pending_op_slot = Some cap \<longrightarrow> \<not> is_pending_cap cap)\<rbrace>
+   set_object a x
+   \<lbrace>\<lambda>_. no_pending\<rbrace>"
   apply (clarsimp simp: set_object_def simpler_modify_def valid_def no_pending_def)
   apply (drule_tac x=oid in spec)
   apply (fastforce simp: opt_cap_def slots_of_def ran_def
@@ -1059,27 +918,26 @@ lemma default_cap_not_pending[simp]:
   by (simp add: default_cap_def is_pending_cap_def split: cdl_object_type.splits)
 
 lemma set_cap_no_pending[wp]:
-  "snd slot = tcb_pending_op_slot \<longrightarrow> \<not> is_pending_cap cap \<Longrightarrow>
-  \<lbrace>no_pending\<rbrace> set_cap slot cap \<lbrace>\<lambda>rv s. no_pending s\<rbrace>"
+  "snd slot = tcb_pending_op_slot \<longrightarrow> \<not> is_pending_cap cap \<Longrightarrow> set_cap slot cap \<lbrace>no_pending\<rbrace>"
   apply (simp add: set_cap_def)
   apply (cases slot, simp)
+  apply (rename_tac oid' idx)
   apply (wp set_object_no_pending | wpc | simp add: no_pending_def)+
-  apply (drule_tac x = a in spec)
+  apply (drule_tac x = oid' in spec)
   apply (rule conjI)
-    apply (clarsimp simp: tcb_pending_op_slot_def tcb_ipcbuffer_slot_def)
+   apply (clarsimp simp: tcb_pending_op_slot_def tcb_ipcbuffer_slot_def)
   apply clarsimp
-  apply (intro conjI impI allI)
-            apply (clarsimp simp: opt_cap_def slots_of_def)+
-            apply (case_tac y, (fastforce simp: object_slots_def update_slots_def)+)
-           apply (clarsimp simp: opt_cap_def slots_of_def)+
+  apply (rename_tac obj)
+  apply (intro conjI impI allI; clarsimp simp: opt_cap_def slots_of_def)
+  apply (case_tac obj; fastforce simp: object_slots_def update_slots_def)
   done
 
 crunch create_cap
   for no_pending[wp]: no_pending
 
 lemma default_object_no_pending_cap:
-  "\<lbrakk> default_object b c d = Some x2; object_slots x2 tcb_pending_op_slot = Some cap\<rbrakk>
-    \<Longrightarrow> \<not> is_pending_cap cap"
+  "\<lbrakk> default_object b c d = Some obj; object_slots obj tcb_pending_op_slot = Some cap\<rbrakk>
+   \<Longrightarrow> \<not> is_pending_cap cap"
   apply (case_tac b)
   apply (clarsimp simp: default_object_def object_slots_def default_tcb_def is_pending_cap_def
                         empty_cnode_def empty_cap_map_def empty_irq_node_def
@@ -1094,7 +952,6 @@ lemma create_objects_no_pending[wp]:
   apply (clarsimp simp: opt_cap_def default_object_no_pending_cap slots_of_def
                  split: if_splits option.split_asm)
   done
-
 
 crunch retype_region
   for no_pending[wp]: "no_pending"
@@ -1114,8 +971,9 @@ lemma is_pending_cap_set_available_range[simp]:
 lemma reset_untyped_cap_no_pending[wp]:
   "\<lbrace>no_pending \<rbrace> reset_untyped_cap cref \<lbrace>\<lambda>rv. no_pending\<rbrace>"
   apply (simp add: reset_untyped_cap_def)
-  apply (wp whenE_wp)
-      apply (rule_tac P = "snd cref = tcb_pending_op_slot \<longrightarrow> \<not> is_pending_cap cap" in hoare_gen_asmEx)
+  apply wp
+      apply (rule_tac P = "snd cref = tcb_pending_op_slot \<longrightarrow> \<not> is_pending_cap cap"
+                      in hoare_gen_asmEx)
       apply (wp mapME_x_inv_wp | simp)+
   apply (clarsimp simp: detype_no_pending)
   apply (cases cref, clarsimp simp: no_pending_def)
@@ -1192,30 +1050,23 @@ lemma invoke_untyped_no_pending[wp]:
   done
 
 lemma is_pending_cap_reset_cap_asid:
-  "reset_cap_asid c = reset_cap_asid c'
-  \<Longrightarrow> is_pending_cap c = is_pending_cap c'"
-  apply (case_tac c')
-  apply (clarsimp simp: is_pending_cap_def dest!:reset_cap_asid_simps2)+
-  done
+  "reset_cap_asid c = reset_cap_asid c' \<Longrightarrow> is_pending_cap c = is_pending_cap c'"
+  by (case_tac c'; clarsimp simp: is_pending_cap_def dest!:reset_cap_asid_simps2)
 
-lemmas
-  is_pending_cap_simps[simp] = is_pending_cap_def[split_simps cdl_cap.split]
+lemmas is_pending_cap_simps[simp] = is_pending_cap_def[split_simps cdl_cap.split]
 
 lemma map_nonempty_split: "xs \<noteq> [] \<Longrightarrow> map f xs = f (hd xs)# map f (tl xs)"
   by (induct xs; clarsimp)
 
-lemma zip_generate_range_single: "\<lbrakk>type \<noteq> UntypedType; n \<noteq> 0\<rbrakk>
-   \<Longrightarrow> zip [x] (generate_range start type sz n) = [(x, {start})]"
+lemma zip_generate_range_single:
+  "\<lbrakk>type \<noteq> UntypedType; n \<noteq> 0\<rbrakk> \<Longrightarrow> zip [x] (generate_range start type sz n) = [(x, {start})]"
   apply (simp add: generate_range_def comp_def)
-  apply (case_tac " [0..<n] = []")
-   apply (simp add: map_nonempty_split)+
+  apply (case_tac "[0..<n] = []"; simp add: map_nonempty_split)
   done
 
 lemma create_cap_touch_wp:
-  "\<lbrace>< (fst xs) \<mapsto>c - \<and>* R >\<rbrace>
-  create_cap new_type sz parent_slot dev xs
-  \<lbrace>\<lambda>_. < (fst xs) \<mapsto>c - \<and>* R >\<rbrace>"
-  apply (simp add: create_cap_def)
+  "create_cap new_type sz parent_slot dev xs \<lbrace>< (fst xs) \<mapsto>c - \<and>* R >\<rbrace>"
+  unfolding create_cap_def
   apply wpc
    apply (wp set_parent_wp)
      apply (wp sep_wp: set_cap_wp)+
@@ -1223,19 +1074,19 @@ lemma create_cap_touch_wp:
   apply sep_solve
   done
 
-lemma sep_map_list_conjD: "\<lbrakk>(\<And>* map P xs) s; \<And>v s. \<lbrakk>v \<in> set xs; P v s\<rbrakk> \<Longrightarrow> P' v s\<rbrakk>
+lemma sep_map_list_conjD:
+  "\<lbrakk>(\<And>* map P xs) s; \<And>v s. \<lbrakk>v \<in> set xs; P v s\<rbrakk> \<Longrightarrow> P' v s\<rbrakk>
    \<Longrightarrow> (\<And>* map P' xs) s"
   apply (induction xs arbitrary: s; simp)
   apply (erule sep_conj_impl; simp)
   done
 
 lemma create_objects_touch_wp:
-  notes set_map[simp del]
-  shows
   "\<lbrace> K (obj_refs = map (\<lambda>x. {x}) (map pick obj_refs) \<and> distinct (map pick obj_refs) \<and> obj \<noteq> None)
      and <(\<And>* ptr\<in>set (map pick obj_refs). ptr \<mapsto>o -) \<and>* P > \<rbrace>
    create_objects obj_refs (obj)
    \<lbrace>\<lambda>r s. <(\<And>* ptr\<in>set (map pick obj_refs). ptr \<mapsto>o -) \<and>* P > s \<rbrace>"
+  supply set_map[simp del]
   apply (rule hoare_name_pre_state, clarsimp)
   apply (subst create_objects_mapM_x'[where ids' = "map pick obj_refs"])
    apply simp
@@ -1246,7 +1097,7 @@ lemma create_objects_touch_wp:
    apply (subst sep_list_conj_sep_map_set_conj[symmetric])
     apply (simp add:distinct_map)
    apply simp
-   apply (clarsimp simp: set_map[symmetric])
+   apply (clarsimp simp flip: set_map)
    apply (subst(asm) sep_list_conj_sep_map_set_conj[symmetric])
     apply (simp add:distinct_map)
    apply (simp add:set_map)
@@ -1261,34 +1112,37 @@ lemma create_objects_touch_wp:
   apply (sep_solve)
   done
 
-lemma retype_region_touch_wp: "\<lbrace>\<lambda>s. obj_refs = map ((\<lambda>x. {x}) \<circ> pick) obj_refs \<and>
-  distinct (map pick obj_refs) \<and> target_type \<noteq> UntypedType \<and> <(\<And>* ptr\<in>set (map pick obj_refs). ptr \<mapsto>o -) \<and>* P> s\<rbrace>
+lemma retype_region_touch_wp:
+  "\<lbrace>\<lambda>s. obj_refs = map ((\<lambda>x. {x}) \<circ> pick) obj_refs \<and>
+        distinct (map pick obj_refs) \<and>
+        target_type \<noteq> UntypedType \<and>
+        <(\<And>* ptr\<in>set (map pick obj_refs). ptr \<mapsto>o -) \<and>* P> s\<rbrace>
    retype_region target_bits target_type obj_refs
-  \<lbrace>\<lambda>r. <(\<And>* ptr\<in>set (map pick obj_refs). ptr \<mapsto>o -) \<and>* P>\<rbrace>"
-  apply (clarsimp simp: retype_region_def, wp)
-    apply(rule create_objects_touch_wp[simplified, THEN sep_lift_generic, simplified])
-   apply (wp)
-  apply (clarsimp)
-  apply (intro conjI)
+   \<lbrace>\<lambda>_. <(\<And>* ptr\<in>set (map pick obj_refs). ptr \<mapsto>o -) \<and>* P>\<rbrace>"
+  apply (clarsimp simp: retype_region_def)
+  apply (wpsimp wp: create_objects_touch_wp[simplified, THEN sep_lift_generic, simplified])
+  apply (rule conjI)
    apply (cases target_type; clarsimp simp: default_object_def)
-  apply (sep_solve)
+  apply sep_solve
   done
 
-lemma update_available_range_touch_wp: "\<lbrace>\<lambda>s. <cap_ref \<mapsto>c - \<and>* P> s\<rbrace>
-  update_available_range ptr idx cap_ref cap
-  \<lbrace>\<lambda>r s. <cap_ref \<mapsto>c - \<and>* P> s\<rbrace>"
+lemma update_available_range_touch_wp:
+  "\<lbrace><cap_ref \<mapsto>c - \<and>* P>\<rbrace>
+   update_available_range ptr idx cap_ref cap
+   \<lbrace>\<lambda>_. <cap_ref \<mapsto>c - \<and>* P>\<rbrace>"
   apply (clarsimp simp: update_available_range_def Let_unfold update_range_def)
   apply (intro conjI impI; wp sep_wp: set_cap_wp, sep_solve)
   done
 
 lemma invoke_untyped_touch_wp:
-  "invocation = (Retype uref nt (unat ts) [dest_slot] has_kids (Suc 0)) \<Longrightarrow>
-   \<lbrace>\<lambda>s. (\<not> has_kids \<longrightarrow> obj_range = free_range) \<and> nt \<noteq> UntypedType \<and>
-    < dest_slot \<mapsto>c NullCap \<and>* uref \<mapsto>c UntypedCap dev obj_range free_range \<and>*
-    (if has_kids then (alignUp (Min (get_range ((\<noteq>) {}) free_range obj_range)) (obj_bits_cdl nt (unat ts))) else  (Min (get_range ((\<noteq>) {}) free_range obj_range))) \<mapsto>o - \<and>*  R> s \<rbrace>
-    invoke_untyped invocation
-   \<lbrace>\<lambda>rv s. <uref \<mapsto>c - \<and>* dest_slot \<mapsto>c - \<and>*
-    (if has_kids then (alignUp (Min (get_range ((\<noteq>) {}) free_range obj_range)) (obj_bits_cdl nt (unat ts))) else  (Min (get_range ((\<noteq>) {}) free_range obj_range))) \<mapsto>o - \<and>* R> s\<rbrace>"
+  "invocation = Retype uref nt (unat ts) [dest_slot] has_kids (Suc 0) \<Longrightarrow>
+   \<lbrace>\<lambda>s. (\<not>has_kids \<longrightarrow> obj_range = free_range) \<and> nt \<noteq> UntypedType \<and>
+        <dest_slot \<mapsto>c NullCap \<and>*
+         uref \<mapsto>c UntypedCap dev obj_range free_range \<and>*
+         (cond_min_of has_kids free_range obj_range nt (unat ts)) \<mapsto>o - \<and>* R> s \<rbrace>
+   invoke_untyped invocation
+   \<lbrace>\<lambda>_. <uref \<mapsto>c - \<and>* dest_slot \<mapsto>c - \<and>*
+         (cond_min_of has_kids free_range obj_range nt (unat ts)) \<mapsto>o - \<and>* R>\<rbrace>"
   apply (rule hoare_name_pre_state)
   apply (clarsimp simp:  invoke_untyped_def)
   apply (intro conjI impI; clarsimp)
@@ -1327,13 +1181,15 @@ lemma invoke_untyped_touch_wp:
   done
 
 lemma invoke_untyped_touch_wp_R:
-  "invocation = (Retype uref nt (unat ts) [dest_slot] has_kids (Suc 0)) \<Longrightarrow>
-   \<lbrace>\<lambda>s. (\<not> has_kids \<longrightarrow> obj_range = free_range) \<and> nt \<noteq> UntypedType \<and>
-    < dest_slot \<mapsto>c NullCap \<and>* uref \<mapsto>c UntypedCap dev obj_range free_range \<and>*
-    (if has_kids then (alignUp (Min (get_range ((\<noteq>) {}) free_range obj_range)) (obj_bits_cdl nt (unat ts))) else  (Min (get_range ((\<noteq>) {}) free_range obj_range))) \<mapsto>o - \<and>*  R> s \<rbrace>
-    invoke_untyped invocation
-   \<lbrace>\<lambda>rv s. <uref \<mapsto>c - \<and>* dest_slot \<mapsto>c - \<and>*
-    (if has_kids then (alignUp (Min (get_range ((\<noteq>) {}) free_range obj_range)) (obj_bits_cdl nt (unat ts))) else  (Min (get_range ((\<noteq>) {}) free_range obj_range))) \<mapsto>o - \<and>* R> s\<rbrace>, -"
+  "invocation = Retype uref nt (unat ts) [dest_slot] has_kids (Suc 0) \<Longrightarrow>
+   \<lbrace>\<lambda>s. (\<not>has_kids \<longrightarrow> obj_range = free_range) \<and> nt \<noteq> UntypedType \<and>
+        <dest_slot \<mapsto>c NullCap \<and>*
+         uref \<mapsto>c UntypedCap dev obj_range free_range \<and>*
+         (cond_min_of has_kids free_range obj_range nt (unat ts)) \<mapsto>o - \<and>*  R> s \<rbrace>
+   invoke_untyped invocation
+   \<lbrace>\<lambda>_. <uref \<mapsto>c - \<and>*
+         dest_slot \<mapsto>c - \<and>*
+         (cond_min_of has_kids free_range obj_range nt (unat ts)) \<mapsto>o - \<and>* R>\<rbrace>, -"
   apply (simp only:)
   apply (rule valid_validE_R)
   apply (rule hoare_chain[OF invoke_untyped_touch_wp])
@@ -1341,119 +1197,123 @@ lemma invoke_untyped_touch_wp_R:
    apply assumption+
   done
 
-abbreviation (input) "retype_with_kids uinv
-  \<equiv> (case uinv of (InvokeUntyped (Retype uref nt ts dest has_kids n)) \<Rightarrow> has_kids)"
+abbreviation (input) retype_with_kids :: "cdl_invocation \<Rightarrow> bool" where
+  "retype_with_kids uinv \<equiv>
+     case uinv of (InvokeUntyped (Retype uref nt ts dest has_kids n)) \<Rightarrow> has_kids"
 
 lemma seL4_Untyped_Retype_inc_no_preempt:
-  "\<lbrakk>cap_object root_cnode_cap = root_cnode;
-   ucptr_slot = offset ucptr root_size;
-   is_cnode_cap root_cnode_cap;
-   ncptr_slot = offset ncptr root_size;
-   unat ncptr_slot_nat = ncptr_slot;
-   one_lvl_lookup root_cnode_cap 32 root_size;
-   guard_equal root_cnode_cap ucptr 32;
-   guard_equal root_cnode_cap croot 32\<rbrakk>
-  \<Longrightarrow> \<lbrace> K (nt\<noteq> UntypedType \<and> default_object  nt (unat ts) minBound = Some obj) and
-    \<guillemotleft>root_tcb_id \<mapsto>f (Tcb tcb)
-  \<and>* (root_tcb_id, tcb_pending_op_slot) \<mapsto>c RunningCap
-  \<and>* (cap_object root_cnode_cap \<mapsto>f CNode (empty_cnode root_size))
-  \<and>* (root_cnode, ucptr_slot) \<mapsto>c UntypedCap dev obj_range free_range
-  \<and>* (root_cnode, ncptr_slot ) \<mapsto>c NullCap
-  \<and>* (\<And>* ptr\<in>tot_free_range. ptr \<mapsto>o Untyped)
-  \<and>* (root_tcb_id, tcb_cspace_slot) \<mapsto>c root_cnode_cap
-  \<and>* (cap_object root_cnode_cap, offset croot root_size) \<mapsto>c root_cnode_cap
-  \<and>* aligned_ptr \<mapsto>o -
-  \<and>* P\<guillemotright>
-    and (\<lambda>s. if has_children (root_cnode,ucptr_slot) (kernel_state s)
-       then  aligned_ptr = alignUp (Min (get_range ((\<noteq>) {}) free_range obj_range)) (obj_bits_cdl nt (unat ts))
-       else obj_range = free_range \<and>  aligned_ptr = Min (get_range ((\<noteq>) {}) free_range obj_range ))
-    and (\<lambda>s. cdl_cdt (kernel_state s) child = Some parent)
-  \<rbrace>
-  seL4_Untyped_Retype ucptr nt ts croot node_index 0 ncptr_slot_nat 1
-  \<lbrace>\<lambda>rv s. cdl_cdt (kernel_state s) child = Some parent\<rbrace>"
-  apply (simp add:seL4_Untyped_Retype_def sep_state_projection2_def)
+  "\<lbrakk> cap_object root_cnode_cap = root_cnode;
+     ucptr_slot = offset ucptr root_size;
+     is_cnode_cap root_cnode_cap;
+     ncptr_slot = offset ncptr root_size;
+     unat ncptr_slot_nat = ncptr_slot;
+     one_lvl_lookup root_cnode_cap 32 root_size;
+     guard_equal root_cnode_cap ucptr 32;
+     guard_equal root_cnode_cap croot 32 \<rbrakk> \<Longrightarrow>
+   \<lbrace> K (nt \<noteq> UntypedType \<and> default_object  nt (unat ts) minBound = Some obj) and
+     \<guillemotleft>root_tcb_id \<mapsto>f (Tcb tcb)
+      \<and>* (root_tcb_id, tcb_pending_op_slot) \<mapsto>c RunningCap
+      \<and>* (cap_object root_cnode_cap \<mapsto>f CNode (empty_cnode root_size))
+      \<and>* (root_cnode, ucptr_slot) \<mapsto>c UntypedCap dev obj_range free_range
+      \<and>* (root_cnode, ncptr_slot ) \<mapsto>c NullCap
+      \<and>* (\<And>* ptr\<in>tot_free_range. ptr \<mapsto>o Untyped)
+      \<and>* (root_tcb_id, tcb_cspace_slot) \<mapsto>c root_cnode_cap
+      \<and>* (cap_object root_cnode_cap, offset croot root_size) \<mapsto>c root_cnode_cap
+      \<and>* aligned_ptr \<mapsto>o -
+      \<and>* P\<guillemotright> and
+     (\<lambda>s. if has_children (root_cnode,ucptr_slot) (kernel_state s)
+          then aligned_ptr = aligned_min_of free_range obj_range nt (unat ts)
+          else obj_range = free_range \<and> aligned_ptr = min_of_range free_range obj_range) and
+     (\<lambda>s. cdl_cdt (kernel_state s) child = Some parent) \<rbrace>
+   seL4_Untyped_Retype ucptr nt ts croot node_index 0 ncptr_slot_nat 1
+   \<lbrace>\<lambda>_ s. cdl_cdt (kernel_state s) child = Some parent\<rbrace>"
+  apply (simp add: seL4_Untyped_Retype_def sep_state_projection2_def)
   apply (rule hoare_name_pre_state)
   apply (rule hoare_pre)
    apply (rule do_kernel_op_pull_back)
-   apply (rule_tac ?Pd2.0="\<lambda>s'. has_children (root_cnode,ucptr_slot) ( s') = has_children (root_cnode,ucptr_slot) (kernel_state s) \<and> Q s'" for Q
-          in call_kernel_with_intent_allow_error_helper[where check= False and tcb = tcb and Q = Q and Perror = Q for Q,simplified])
+   apply (rule_tac ?Pd2.0="\<lambda>s'. has_children (root_cnode, ucptr_slot) s' =
+                                has_children (root_cnode, ucptr_slot) (kernel_state s)
+                                \<and> Q s'" for Q
+                   in call_kernel_with_intent_allow_error_helper[where
+                        check= False and tcb = tcb and Q = Q and Perror = Q for Q,simplified])
                apply fastforce
-              apply (wp)+
-         apply (rule_tac P = "\<exists>has_kids. iv = InvokeUntyped (Retype (root_cnode,ucptr_slot) nt (unat ts)
-               [(root_cnode, ncptr_slot)]
-               has_kids 1)"
-           in hoare_gen_asmEx)
+              apply wp+
+         apply (rule_tac P = "\<exists>has_kids. iv = InvokeUntyped (Retype (root_cnode, ucptr_slot)
+                                                                    nt
+                                                                    (unat ts)
+                                                                    [(root_cnode, ncptr_slot)]
+                                                                    has_kids 1)"
+                         in hoare_gen_asmEx)
          apply clarsimp
-         apply (rule hoare_vcg_conj_elimE[where P = P and P' = P for P,simplified,rotated])
+         apply (rule hoare_vcg_conj_elimE[where P = P and P' = P for P, simplified, rotated])
           apply wp
           apply (rule hoare_strengthen_postE_R[OF hoare_vcg_conj_liftE_R])
             apply (rule valid_validE_R)
             apply (rule invoke_untyped_cdt_inc)
            apply (rule invoke_untyped_touch_wp_R [where
-                        uref = "(cap_object root_cnode_cap, offset ucptr root_size)"
-                    and dest_slot = "(cap_object root_cnode_cap, offset ncptr root_size)"
-                    and free_range = free_range and nt=nt and ts="ts"
-                    and obj_range = obj_range, simplified sep_wp_simp, THEN sep_lift_generic_R])
+                            uref = "(cap_object root_cnode_cap, offset ucptr root_size)"
+                         and dest_slot = "(cap_object root_cnode_cap, offset ncptr root_size)"
+                         and free_range = free_range
+                         and nt = nt
+                         and ts = ts
+                         and obj_range = obj_range,
+                         simplified sep_wp_simp, THEN sep_lift_generic_R])
            apply clarsimp
-           apply (rule_tac s="retype_with_kids (InvokeUntyped (Retype _ _ _ _ has_kids _))" in trans, simp, rule refl)
+           apply (rule_tac s="retype_with_kids (InvokeUntyped (Retype _ _ _ _ has_kids _))" in trans,
+                  simp, rule refl)
           apply clarsimp
           apply (rule conjI)
            apply (sep_erule refl_imp, simp)
           apply fastforce
          apply (rule hoare_pre)
-          apply (rule invoke_untyped_exception[where  free_range = free_range and obj_range = obj_range], simp)
-         apply (clarsimp)
-         apply (sep_solve)
+          apply (rule invoke_untyped_exception[where free_range = free_range and
+                                                     obj_range = obj_range],
+                 simp)
+         apply clarsimp
+         apply sep_solve
         apply (wp hoare_vcg_conj_lift)
          apply (wp hoare_strengthen_post[OF set_cap_wp])
-         apply (sep_schem)
-        apply wp[1]
-       apply (rule_tac P ="nt \<noteq> UntypedType \<and> c = UntypedCap dev obj_range free_range \<and> cs = [(root_cnode_cap,(root_cnode,offset croot root_size))]"
-        in hoare_gen_asmEx)
+         apply sep_schem
+        apply wp
+       apply (rule_tac P = "nt \<noteq> UntypedType \<and> c = UntypedCap dev obj_range free_range \<and>
+                            cs = [(root_cnode_cap, (root_cnode, offset croot root_size))]"
+                       in hoare_gen_asmEx)
        apply simp
        apply (rule decode_untyped_invocation_rvu)
        apply simp
-      apply (simp add:lookup_extra_caps_def mapME_singleton)
+      apply (simp add: lookup_extra_caps_def mapME_singleton)
       apply (rule wp_no_exception_seq)
-       apply wp[1]
+       apply wp
       apply (rule lookup_cap_and_slot_rvu[where r = root_size and  cap' = "root_cnode_cap"])
      apply clarsimp
      apply (rule hoare_weaken_preE)
-      apply (rule lookup_cap_and_slot_rvu[where r = root_size and cap' = "UntypedCap dev obj_range free_range"])[1]
-     apply (force)
-    apply (wp hoare_vcg_ball_lift
-              update_thread_intent_update
+      apply (rule lookup_cap_and_slot_rvu[where r = root_size and
+                                                cap' = "UntypedCap dev obj_range free_range"])
+     apply force
+    apply (wp hoare_vcg_ball_lift update_thread_intent_update
               hoare_vcg_imp_lift hoare_vcg_ex_lift hoare_vcg_all_lift
               is_cnode_cap_guard_equal update_thread_intent_update)
-   apply clarsimp+
-   apply (case_tac "has_children (cap_object root_cnode_cap, offset ucptr root_size) sa", clarsimp)
+   apply (rename_tac s')
+   apply clarsimp
+   apply (case_tac "has_children (cap_object root_cnode_cap, offset ucptr root_size) s'", clarsimp)
     apply (drule mp, force)
-    apply (clarsimp)
-    apply (sep_schem)
+    apply clarsimp
+    apply sep_schem
    apply (drule mp, force)
-   apply (clarsimp)
-   apply (sep_schem)
-  apply (clarsimp)
+   apply clarsimp
+   apply sep_schem
+  apply clarsimp
   apply (intro conjI impI)
-         apply (erule conjE)+
          apply clarsimp
-         apply (sep_cancel)
-         apply (sep_cancel)
-         apply (sep_cancel)
-         apply (sep_cancel)
-         apply (sep_cancel)
-         apply (sep_cancel)
+         apply (repeat 6 sep_cancel)
          apply (sep_erule refl_imp)
          apply (rule TrueI)
-        apply (sep_solve)+
-       apply (erule conjE)+
-       apply (fastforce)
+        apply sep_solve+
+       apply fastforce
       apply (subst disj_imp, intro impI conjI)
-         apply (clarsimp)
-        apply (clarsimp, sep_solve)
-       apply (clarsimp)
-       apply (clarsimp simp: user_pointer_at_def Let_def ep_related_cap_def
-                                       word_bits_def sep_conj_assoc
-                                dest!: reset_cap_asid_simps2 reset_cap_asid_cnode_cap | sep_solve)+
+         apply (clarsimp simp: user_pointer_at_def Let_def ep_related_cap_def
+                               word_bits_def sep_conj_assoc
+                         dest!: reset_cap_asid_simps2 reset_cap_asid_cnode_cap | sep_solve)+
   done
+
 end
